@prefix dgprops: <http://www.darkglass.com/lv2/ns#> .
@prefix lv2:     <http://lv2plug.in/ns/lv2core#> .
@prefix opts:    <http://lv2plug.in/ns/ext/options#> .
@prefix owl:     <http://www.w3.org/2002/07/owl#> .
@prefix rdf:     <http://www.w3.org/1999/02/22-rdf-syntax-ns#> .
@prefix rdfs:    <http://www.w3.org/2000/01/rdf-schema#> .
@prefix units:   <http://lv2plug.in/ns/extensions/units#> .
@prefix xsd:     <http://www.w3.org/2001/XMLSchema#> .

<http://www.darkglass.com/lv2/ns>
    a owl:Ontology ;
    rdfs:seeAlso <props.h> ,
        <props.doap.ttl> ,
        <../dg-meta/meta.ttl> ;
    rdfs:comment "A set of custom LV2 properties created by and for Darkglass related products." .

dgprops:abbreviation
    a rdf:Property , owl:DatatypeProperty ;
    rdfs:range xsd:string ;
    rdfs:label "abbreviation" ;
    rdfs:comment "Plugin name abbreviation consisting of 2 or 3 characters in uppercase." .

dgprops:blockImageOff
    a rdf:Property , owl:ObjectProperty ;
    rdfs:range owl:Thing ;
    rdfs:label "block image off" ;
    rdfs:comment "Path to a in-bundle/local 200x200 PNG image file to be used as the plugin's block image asset when OFF." .

dgprops:blockImageOn
    a rdf:Property , owl:ObjectProperty ;
    rdfs:range owl:Thing ;
    rdfs:label "block image on" ;
    rdfs:comment "Path to a in-bundle/local  200x200 PNG image file to be used as the plugin's block image asset when ON." .

dgprops:oneDecimalPoint
    a units:Unit ;
    rdfs:label "One Decimal Point" ;
    rdfs:comment "Meaningless unit that forces usage of 1 decimal point." ;
    units:symbol "" ;
    units:render "%.1f" .

dgprops:quickPot
    a rdf:Property , owl:DatatypeProperty ;
    rdfs:range xsd:float ;
    rdfs:label "quick pot" ;
    rdfs:comment "The parameter designated as the Quick Pot for a plugin." .

dgprops:savedToPreset
    a lv2:PortProperty ;
    rdfs:label "saved to preset" ;
    rdfs:comment "Force a parameter or property to be saved to preset." .

dgprops:mayBecomeInactive
    a lv2:PortProperty ;
    rdfs:label "may become inactive" ;
    rdfs:comment "Plugin may report this parameter as inactive (inaudible edits) at run-time." .

dgprops:mayBecomeBlocked
    a lv2:PortProperty ;
    rdfs:label "may become blocked" ;
    rdfs:comment "Plugin may report this parameter as blocked (not allowed) at run-time." .
